Update

src/checker.lean
@@ -6,17 +6,22 @@ section
 
 open expr
 open ctx
-
 open small
 open small_star
-open small_eq
-open has_type
+open defeq
+open judgment_index
+open judgment
 
-local notation e ` ⟦` n ` ↦ ` e' `⟧` := expr.subst e n e'
-local notation e ` ⟦` n ` ↟ ` m `⟧`  := expr.shift e n m
-local notation e ` ~>* ` e'          := small_star e e'
-local notation e ` ~~ ` e'           := small_eq e e'
-local notation Γ ` ▷ ` e ` : ` t     := has_type Γ e t
+set_option pp.beta true
+set_option pp.structure_projections false
+
+local notation e ` ⟦`:80 n:80 ` ↦ `:80 e':79 `⟧`:79 := subst e n e'
+local notation e ` ⟦`:80 n:80 ` ↟ `:80 m:79 `⟧`:79  := shift e n m
+local notation e ` ~> `:50 e':50                    := small e e'
+local notation e ` ~>* `:50 e':50                   := small_star e e'
+local notation e ` ~~ `:50 e':50                    := defeq e e'
+local notation `▷ `:50 Γ:50                         := judgment (well_ctx Γ )
+local notation Γ ` ▷ `:50 e:50 ` : `:50 t:50        := judgment (has_type Γ e t)
 
 /-- Performs applicative-order beta-reduction.
     If the original expression is well-typed, the resulting expression will have the same type.
@@ -31,19 +36,19 @@ meta def expr.reduce : Π (e : expr), Σ' (e' : expr), e ~>* e'
     match l', hl with
     | (lam t e), hl' :=
       let ⟨e', he⟩ := expr.reduce (e ⟦0 ↦ r'⟧) in
-        ⟨e', small_star_trans (ss_step (small_star_app hl' hr) s_beta) he⟩
-    | _,         _   := ⟨app l' r', small_star_app hl hr⟩
+        ⟨e', small_star_trans (ss_step (app_small_star_aux hl' hr) s_beta) he⟩
+    | _,         _   := ⟨app l' r', app_small_star_aux hl hr⟩
     end
 | (lam t e)  :=
   let ⟨t', ht⟩ := expr.reduce t,
       ⟨e', he⟩ := expr.reduce e in
-  ⟨lam t' e', small_star_lam ht he⟩
+  ⟨lam t' e', lam_small_star_aux ht he⟩
 | (pi t₁ t₂) :=
   let ⟨t₁', ht₁⟩ := expr.reduce t₁,
       ⟨t₂', ht₂⟩ := expr.reduce t₂ in
-    ⟨pi t₁' t₂', small_star_pi ht₁ ht₂⟩
+    ⟨pi t₁' t₂', pi_small_star_aux ht₁ ht₂⟩
 
-/- Some helper functions. -/
+/- Helper functions and auxiliary lemmas. -/
 
 def expr.as_sort : Π (e : expr), string ⊕ Σ' (n : nat), e = sort n
 | (sort s) := sum.inr ⟨s, rfl⟩
@@ -58,34 +63,58 @@ def ctx.try_nth : Π (Γ : ctx) (n : nat), string ⊕ Σ' (e : expr), list.nth �
 | (t :: Γ) 0       := sum.inr ⟨t, rfl⟩
 | (t :: Γ) (n + 1) := ctx.try_nth Γ n
 
+lemma expr.check_aux_1
+  {Γ l tl} (htl : Γ ▷ l : tl) {t₁ t₂} (htt : tl = pi t₁ t₂) {r tr} (htr : Γ ▷ r : tr)
+  {t₁'} (ht₁' : t₁ ~>* t₁') {tr'} (htr' : tr ~>* tr') (he : t₁' = tr') :
+  (Γ ▷ app l r : t₂ ⟦0 ↦ r⟧) := by
+{ substs htt he,
+  have h₁ := has_type_conv_small_star htl (pi_small_star_aux ht₁' ss_refl),
+  have h₂ := has_type_conv_small_star htr htr',
+  exact t_app h₁ h₂ }
+
+lemma expr.check_aux_2
+  {Γ t t'} (ht' : Γ ▷ t : t') {s} (hs : t' = sort s) {e t₂} (ht₂ : t :: Γ ▷ e : t₂) :
+  (Γ ▷ lam t e : pi t t₂) := by
+{ subst hs,
+  obtain ⟨s₂, hs₂⟩ := type_has_sort ht₂,
+  exact t_lam (t_pi ht' hs₂) ht₂ }
+
 /-- Check if a preterm is a well-formed term.
     Returns its type and the corresponding proof on success.
     It should terminate on any input, but there is no proof yet. -/
-meta def expr.check : Π (e : expr) (Γ : ctx), string ⊕ Σ' (t : expr), Γ ▷ e : t
-| (sort s)   Γ := return ⟨sort (s + 1), t_sort⟩
-| (var v)    Γ := do ⟨t, h⟩ <- Γ.try_nth v, return ⟨t.shift 0 v.succ, t_var h⟩
-| (app l r)  Γ := do
-  { ⟨tl, htl⟩     ← l.check Γ,
+meta def expr.check : Π (e : expr) (Γ : ctx), ▷ Γ → string ⊕ Σ' (t : expr), Γ ▷ e : t
+| (sort s)   Γ hw := return ⟨sort (s + 1), t_sort hw⟩
+| (var v)    Γ hw := do ⟨t, h⟩ <- Γ.try_nth v, return ⟨t.shift 0 v.succ, t_var hw h⟩
+| (app l r)  Γ hw := do
+  { ⟨tl, htl⟩     ← l.check Γ hw,
     ⟨t₁, t₂, htt⟩ ← tl.as_pi,
-    ⟨tr, htr⟩     ← r.check Γ,
+    ⟨tr, htr⟩     ← r.check Γ hw,
     let ⟨t₁', ht₁'⟩ := t₁.reduce,
     let ⟨tr', htr'⟩ := tr.reduce,
     dite (t₁' = tr')
-      (λ heq, return ⟨t₂.subst 0 r, t_app (t_conv
-        (small_eq_pi (small_eq_of_small_stars (heq ▸ ht₁' : t₁ ~>* tr') htr') se_refl)
-        (htt ▸ htl : Γ ▷ l : pi t₁ t₂)) htr⟩)
+      (λ he, return ⟨t₂ ⟦0 ↦ r⟧, expr.check_aux_1 htl htt htr ht₁' htr' he⟩)
       (λ _, sum.inl $ "argument type mismatch: " ++ t₁.show ++ " != " ++ tr.show) }
-| (lam t e)  Γ := do
-  { ⟨t₂, ht₂⟩     ← e.check (t :: Γ),
-    ⟨t', ht'⟩     ← (pi t t₂).check Γ,
+| (lam t e)  Γ hw := do
+  { ⟨t', ht'⟩     ← t.check Γ hw,
     ⟨s, hs⟩       ← t'.as_sort,
-    return ⟨pi t t₂, t_lam (hs ▸ ht' : Γ ▷ pi t t₂ : sort s) ht₂⟩ }
-| (pi t₁ t₂) Γ := do
-  { ⟨t₁', ht₁'⟩   ← t₁.check Γ,
+    ⟨t₂, ht₂⟩     ← e.check (t :: Γ) (c_cons (hs ▸ ht' : Γ ▷ t : sort s)),
+    return ⟨pi t t₂, expr.check_aux_2 ht' hs ht₂⟩ }
+| (pi t₁ t₂) Γ hw := do
+  { ⟨t₁', ht₁'⟩   ← t₁.check Γ hw,
     ⟨s₁, hs₁⟩     ← t₁'.as_sort,
-    ⟨t₂', ht₂'⟩   ← t₂.check (t₁ :: Γ),
+    ⟨t₂', ht₂'⟩   ← t₂.check (t₁ :: Γ) (c_cons (hs₁ ▸ ht₁' : Γ ▷ t₁ : sort s₁)),
     ⟨s₂, hs₂⟩     ← t₂'.as_sort,
     return ⟨sort (max s₁ s₂), t_pi (hs₁ ▸ ht₁') (hs₂ ▸ ht₂')⟩ }
+
+/-- Check if a precontext is a well-formed context.
+    Returns a proof on success. -/
+meta def ctx.check : Π (Γ : ctx), string ⊕ Σ' (_ : unit), ▷ Γ
+| []       := return ⟨(), c_nil⟩
+| (t :: Γ) := do
+  { ⟨_, hw⟩   ← ctx.check Γ,
+    ⟨t', ht'⟩ ← t.check Γ hw,
+    ⟨s, hs⟩   ← t'.as_sort,
+    return ⟨(), c_cons (hs ▸ ht' : Γ ▷ t : sort s)⟩ }
 
 end
 end coc
